more

thys/POPLmark/SystemFSub.thy
@@ -1,12 +1,12 @@
-(* System F with SubTypeing  *)
+(* System F with SubsftypePing  *)
 theory SystemFSub
   imports "SystemFSub_Types"
 begin
 
-abbreviation in_context :: "var \<Rightarrow> type \<Rightarrow> \<Gamma>\<^sub>\<tau> \<Rightarrow> bool" ("_ <: _ \<in> _" [55,55,55] 60) where
+abbreviation in_context :: "var \<Rightarrow> sftype \<Rightarrow> \<Gamma>\<^sub>\<tau> \<Rightarrow> bool" ("_ <: _ \<in> _" [55,55,55] 60) where
   "x <: t \<in> \<Gamma> \<equiv> (x, t) \<in> set \<Gamma>"
-abbreviation well_scoped :: "type \<Rightarrow> \<Gamma>\<^sub>\<tau> \<Rightarrow> bool" ("_ closed'_in _" [55, 55] 60) where
-  "well_scoped S \<Gamma> \<equiv> FFVars_Type S \<subseteq> dom \<Gamma>"
+abbreviation well_scoped :: "sftype \<Rightarrow> \<Gamma>\<^sub>\<tau> \<Rightarrow> bool" ("_ closed'_in _" [55, 55] 60) where
+  "well_scoped S \<Gamma> \<equiv> FFVars_sftypeP S \<subseteq> dom \<Gamma>"
 
 inductive wf :: "\<Gamma>\<^sub>\<tau> \<Rightarrow> bool"  where
   wf_Nil[intro]: "wf []"
@@ -19,18 +19,18 @@ print_theorems
 
 lemma in_context_eqvt:
   assumes "bij f" "|supp f| <o |UNIV::var set|"
-  shows "x <: T \<in> \<Gamma> \<Longrightarrow> f x <: rrename_Type f T \<in> map_context f \<Gamma>"
+  shows "x <: T \<in> \<Gamma> \<Longrightarrow> f x <: rrename_sftypeP f T \<in> map_context f \<Gamma>"
   using assms unfolding map_context_def by auto
 
 lemma extend_eqvt:
   assumes "bij f" "|supp f| <o |UNIV::var set|"
-  shows "map_context f (\<Gamma>,,x<:T) = map_context f \<Gamma>,,f x <: rrename_Type f T"
+  shows "map_context f (\<Gamma>,,x<:T) = map_context f \<Gamma>,,f x <: rrename_sftypeP f T"
   using assms unfolding map_context_def by simp
 
 lemma closed_in_eqvt:
   assumes "bij f" "|supp f| <o |UNIV::var set|"
-  shows "S closed_in \<Gamma> \<Longrightarrow> rrename_Type f S closed_in map_context f \<Gamma>"
-  using assms by (auto simp: Type.FFVars_rrenames)
+  shows "S closed_in \<Gamma> \<Longrightarrow> rrename_sftypeP f S closed_in map_context f \<Gamma>"
+  using assms by (auto simp: sftypeP.FFVars_rrenames)
 
 lemma wf_eqvt:
   assumes "bij f" "|supp f| <o |UNIV::var set|"
@@ -42,11 +42,11 @@ unfolding map_context_def proof (induction \<Gamma>)
     using closed_in_eqvt map_context_def by fastforce
 qed simp
 
-abbreviation Tsupp :: "\<Gamma>\<^sub>\<tau> \<Rightarrow> type \<Rightarrow> type \<Rightarrow> var set" where
-  "Tsupp \<Gamma> T\<^sub>1 T\<^sub>2 \<equiv> dom \<Gamma> \<union> FFVars_ctxt \<Gamma> \<union> FFVars_Type T\<^sub>1 \<union> FFVars_Type T\<^sub>2"
+abbreviation Tsupp :: "\<Gamma>\<^sub>\<tau> \<Rightarrow> sftype \<Rightarrow> sftype \<Rightarrow> var set" where
+  "Tsupp \<Gamma> T\<^sub>1 T\<^sub>2 \<equiv> dom \<Gamma> \<union> FFVars_ctxt \<Gamma> \<union> FFVars_sftypeP T\<^sub>1 \<union> FFVars_sftypeP T\<^sub>2"
 
 lemma small_Tsupp: "small (Tsupp \<Gamma> T\<^sub>1 T\<^sub>2)"
-  by (auto simp: small_def Type.card_of_FFVars_bounds Type.Un_bound var_Type_pre_class.UN_bound set_bd_UNIV Type.set_bd)
+  by (auto simp: small_def sftypeP.card_of_FFVars_bounds sftypeP.Un_bound var_sftypeP_pre_class.UN_bound set_bd_UNIV sftypeP.set_bd)
 
 lemma fresh: "\<exists>xx. xx \<notin> Tsupp \<Gamma> T\<^sub>1 T\<^sub>2"
   by (metis emp_bound equals0D imageI inf.commute inf_absorb2 small_Tsupp small_def small_isPerm subsetI)
@@ -73,17 +73,17 @@ qed
 
 (* *)
 
-inductive ty :: "\<Gamma>\<^sub>\<tau> \<Rightarrow> type \<Rightarrow> type \<Rightarrow> bool" ("_ \<turnstile> _ <: _" [55,55,55] 60) where
+inductive ty :: "\<Gamma>\<^sub>\<tau> \<Rightarrow> sftype \<Rightarrow> sftype \<Rightarrow> bool" ("_ \<turnstile> _ <: _" [55,55,55] 60) where
   SA_Top: "\<lbrakk>wf \<Gamma>; S closed_in \<Gamma> \<rbrakk> \<Longrightarrow> \<Gamma> \<turnstile> S <: Top"
-| SA_Refl_TVar: "\<lbrakk>wf \<Gamma>; TyVar x closed_in \<Gamma> \<rbrakk> \<Longrightarrow> \<Gamma> \<turnstile> TyVar x <: TyVar x"
-| SA_Trans_TVar: "\<lbrakk> X<:U \<in> \<Gamma> ; \<Gamma> \<turnstile> U <: T \<rbrakk> \<Longrightarrow> \<Gamma> \<turnstile> TyVar X <: T"
+| SA_Refl_TVar: "\<lbrakk>wf \<Gamma>; TVr x closed_in \<Gamma> \<rbrakk> \<Longrightarrow> \<Gamma> \<turnstile> TVr x <: TVr x"
+| SA_Trans_TVar: "\<lbrakk> X<:U \<in> \<Gamma> ; \<Gamma> \<turnstile> U <: T \<rbrakk> \<Longrightarrow> \<Gamma> \<turnstile> TVr X <: T"
 | SA_Arrow: "\<lbrakk> \<Gamma> \<turnstile> T\<^sub>1 <: S\<^sub>1 ; \<Gamma> \<turnstile> S\<^sub>2 <: T\<^sub>2 \<rbrakk> \<Longrightarrow> \<Gamma> \<turnstile> S\<^sub>1 \<rightarrow> S\<^sub>2 <: T\<^sub>1 \<rightarrow> T\<^sub>2"
 | SA_All: "\<lbrakk> \<Gamma> \<turnstile> T\<^sub>1 <: S\<^sub>1 ; \<Gamma>,, X<:T\<^sub>1 \<turnstile> S\<^sub>2 <: T\<^sub>2 \<rbrakk> \<Longrightarrow> \<Gamma> \<turnstile> \<forall>X<:S\<^sub>1. S\<^sub>2 <: \<forall>X<:T\<^sub>1 .T\<^sub>2"
 
 inductive_cases
   SA_TopE[elim!]: "\<Gamma> \<turnstile> Top <: T"
 and
-  SA_TVarE: "\<Gamma> \<turnstile> S <: TyVar Z"
+  SA_TVarE: "\<Gamma> \<turnstile> S <: TVr Z"
 and
   SA_ArrER: "\<Gamma> \<turnstile> S <: T\<^sub>1 \<rightarrow> T\<^sub>2"
 and
@@ -102,24 +102,24 @@ lemma well_scoped:
 using assms proof (induction \<Gamma> S T rule: ty.induct)
 case (SA_Trans_TVar x U \<Gamma> T) {
   case 1 then show ?case using SA_Trans_TVar
-    by (metis fst_conv imageI singletonD subsetI Type.set(1))
+    by (metis fst_conv imageI singletonD subsetI sftypeP.set(1))
 next
   case 2 then show ?case using SA_Trans_TVar by simp
 } qed auto
 
 declare ty.intros[intro]
 
-lemma ty_fresh_extend: "\<Gamma>,, x <: U \<turnstile> S <: T \<Longrightarrow> x \<notin> dom \<Gamma> \<union> FFVars_ctxt \<Gamma> \<and> x \<notin> FFVars_Type U"
+lemma ty_fresh_extend: "\<Gamma>,, x <: U \<turnstile> S <: T \<Longrightarrow> x \<notin> dom \<Gamma> \<union> FFVars_ctxt \<Gamma> \<and> x \<notin> FFVars_sftypeP U"
   by (metis (no_types, lifting) UnE fst_conv snd_conv subsetD wf_ConsE wf_FFVars wf_context)
 
 make_binder_inductive ty
   subgoal for R B \<sigma> \<Gamma> T1 T2
     unfolding split_beta
     by (elim disj_forward exE)
-      (auto simp add: isPerm_def supp_inv_bound map_context_def[symmetric] Type_vvsubst_rrename
-        Type.rrename_comps Type.FFVars_rrenames wf_eqvt extend_eqvt
+      (auto simp add: isPerm_def supp_inv_bound map_context_def[symmetric] sftypeP_vvsubst_rrename
+        sftypeP.rrename_comps sftypeP.FFVars_rrenames wf_eqvt extend_eqvt
         | ((rule exI[of _ "\<sigma> _"] exI)+, (rule conjI)?, rule refl)
-        | ((rule exI[of _ "rrename_Type \<sigma> _"])+, (rule conjI)?, rule in_context_eqvt))+
+        | ((rule exI[of _ "rrename_sftypeP \<sigma> _"])+, (rule conjI)?, rule in_context_eqvt))+
   subgoal premises prems for R B \<Gamma> T1 T2
     using prems
     unfolding ex_push_inwards conj_disj_distribL ex_disj_distrib
@@ -144,7 +144,7 @@ make_binder_inductive ty
          apply (drule prems(2)[rule_format, of "id(X := Z, Z := X)" "\<Gamma>,, X <: T\<^sub>1" "S\<^sub>2" "T\<^sub>2", rotated 2])
            apply (auto simp: extend_eqvt)
         apply(rule cong[OF cong[OF cong], THEN iffD1, of R , OF refl, rotated -1, 
-          of _ "rrename_Type (id(X := Z, Z := X)) S\<^sub>2"]) 
+          of _ "rrename_sftypeP (id(X := Z, Z := X)) S\<^sub>2"]) 
           apply (drule ty_fresh_extend)
           apply (simp_all add: supp_swap_bound)
           by (metis (no_types, opaque_lifting) image_iff map_context_def map_context_swap_FFVars)
