thys/POPLmark/SystemFSub_Types.thy
@@ -1,4 +1,4 @@
-(* Types for System F with SubTypeing  *)
+(* sftypePs for System F with SubsftypePing  *)
 theory SystemFSub_Types
   imports "Binders.MRBNF_Recursor"
     "Binders.Generic_Strong_Rule_Induction"
@@ -13,73 +13,73 @@ declare supp_id_bound[simp]
 (*type_synonym label = nat*)
 
 declare [[mrbnf_internals]]
-binder_datatype 'var "Type" =
-    TyVar 'var
+binder_datatype 'tvar "sftypeP" =
+    TVr 'tvar
   | Top
-  | Fun "'var Type" "'var Type"
-  | Forall X::'var "'var Type" T::"'var Type" binds X in T
+  | Fun "'tvar sftypeP" "'tvar sftypeP"
+  | Forall X::'tvar "'tvar sftypeP" T::"'tvar sftypeP" binds X in T
 
-declare supp_swap_bound[OF cinfinite_imp_infinite[OF Type.UNIV_cinfinite], simp]
-declare Type.rrename_ids[simp] Type.rrename_id0s[simp]
+declare supp_swap_bound[OF cinfinite_imp_infinite[OF sftypeP.UNIV_cinfinite], simp]
+declare sftypeP.rrename_ids[simp] sftypeP.rrename_id0s[simp]
 
-lemma rrename_Type_simps[simp]:
-  fixes f::"'a::var_Type_pre \<Rightarrow> 'a"
+lemma rrename_sftypeP_simps[simp]:
+  fixes f::"'a::var_sftypeP_pre \<Rightarrow> 'a"
   assumes "bij f" "|supp f| <o |UNIV::'a set|"
   shows
-    "rrename_Type f (TyVar X) = TyVar (f X)"
-    "rrename_Type f Top = Top"
-    "rrename_Type f (Fun t1 t2) = Fun (rrename_Type f t1) (rrename_Type f t2)"
-    "rrename_Type f (Forall Y T1 T2) = Forall (f Y) (rrename_Type f T1) (rrename_Type f T2)"
-     apply (unfold TyVar_def Top_def Fun_def Forall_def)
+    "rrename_sftypeP f (TVr X) = TVr (f X)"
+    "rrename_sftypeP f Top = Top"
+    "rrename_sftypeP f (Fun t1 t2) = Fun (rrename_sftypeP f t1) (rrename_sftypeP f t2)"
+    "rrename_sftypeP f (Forall Y T1 T2) = Forall (f Y) (rrename_sftypeP f T1) (rrename_sftypeP f T2)"
+     apply (unfold TVr_def Top_def Fun_def Forall_def)
      apply (rule trans)
-      apply (rule Type.rrename_cctors)
+      apply (rule sftypeP.rrename_cctors)
        apply (rule assms)+
      defer
      apply (rule trans)
-      apply (rule Type.rrename_cctors)
+      apply (rule sftypeP.rrename_cctors)
        apply (rule assms)+
      defer
      apply (rule trans)
-      apply (rule Type.rrename_cctors)
+      apply (rule sftypeP.rrename_cctors)
        apply (rule assms)+
      defer
      apply (rule trans)
-      apply (rule Type.rrename_cctors)
+      apply (rule sftypeP.rrename_cctors)
        apply (rule assms)+
      defer
-     apply (unfold map_Type_pre_def comp_def Abs_Type_pre_inverse[OF UNIV_I] map_sum.simps
+     apply (unfold map_sftypeP_pre_def comp_def Abs_sftypeP_pre_inverse[OF UNIV_I] map_sum.simps
         map_prod_simp id_def
       )
      apply (rule refl)+
   done
 
-lemma Type_inject:
-  "TyVar X = TyVar Y \<longleftrightarrow> X = Y"
+lemma sftypeP_inject:
+  "TVr X = TVr Y \<longleftrightarrow> X = Y"
   "Fun T1 T2 = Fun R1 R2 \<longleftrightarrow> T1 = R1 \<and> T2 = R2"
   "Forall X T1 T2 = Forall Y R1 R2 \<longleftrightarrow> 
-   T1 = R1 \<and> (\<exists>f. bij (f::'a::var_Type_pre \<Rightarrow> 'a) \<and> 
-   |supp f| <o |UNIV::'a set| \<and> id_on (FFVars_Type T2 - {X}) f \<and> f X = Y \<and> rrename_Type f T2 = R2)"
-    apply (unfold TyVar_def Fun_def Forall_def Type.TT_injects0
-      set3_Type_pre_def comp_def Abs_Type_pre_inverse[OF UNIV_I] map_sum.simps sum_set_simps
-      cSup_singleton Un_empty_left Un_empty_right Union_empty image_empty empty_Diff map_Type_pre_def
-      prod.map_id set2_Type_pre_def prod_set_simps prod.set_map UN_single Abs_Type_pre_inject[OF UNIV_I UNIV_I]
+   T1 = R1 \<and> (\<exists>f. bij (f::'a::var_sftypeP_pre \<Rightarrow> 'a) \<and> 
+   |supp f| <o |UNIV::'a set| \<and> id_on (FFVars_sftypeP T2 - {X}) f \<and> f X = Y \<and> rrename_sftypeP f T2 = R2)"
+    apply (unfold TVr_def Fun_def Forall_def sftypeP.TT_injects0
+      set3_sftypeP_pre_def comp_def Abs_sftypeP_pre_inverse[OF UNIV_I] map_sum.simps sum_set_simps
+      cSup_singleton Un_empty_left Un_empty_right Union_empty image_empty empty_Diff map_sftypeP_pre_def
+      prod.map_id set2_sftypeP_pre_def prod_set_simps prod.set_map UN_single Abs_sftypeP_pre_inject[OF UNIV_I UNIV_I]
       sum.inject prod.inject map_prod_simp
     )
   by auto
-declare Type_inject(1,2)[simp]
+declare sftypeP_inject(1,2)[simp]
 
 corollary Forall_inject_same[simp]: "Forall X T1 T2 = Forall X S1 S2 \<longleftrightarrow> T1 = S1 \<and> T2 = S2"
-  using Type_inject(3) Type.rrename_cong_ids
+  using sftypeP_inject(3) sftypeP.rrename_cong_ids
   by (metis (no_types, lifting) Diff_empty Diff_insert0 id_on_insert insert_Diff)
 
 lemma Forall_rrename:
   assumes "bij \<sigma>" "|supp \<sigma>| <o |UNIV::'a set|" shows "
- (\<And>Y. Y\<in>FFVars_Type T2 - {X::'a::var_Type_pre} \<Longrightarrow> \<sigma> Y = Y) \<Longrightarrow> Forall X T1 T2 = Forall (\<sigma> X) T1 (rrename_Type \<sigma> T2)"
+ (\<And>Y. Y\<in>FFVars_sftypeP T2 - {X::'a::var_sftypeP_pre} \<Longrightarrow> \<sigma> Y = Y) \<Longrightarrow> Forall X T1 T2 = Forall (\<sigma> X) T1 (rrename_sftypeP \<sigma> T2)"
   apply (unfold Forall_def)
-  apply (unfold Type.TT_injects0)
-  apply (unfold set3_Type_pre_def set2_Type_pre_def comp_def Abs_Type_pre_inverse[OF UNIV_I] map_sum.simps
+  apply (unfold sftypeP.TT_injects0)
+  apply (unfold set3_sftypeP_pre_def set2_sftypeP_pre_def comp_def Abs_sftypeP_pre_inverse[OF UNIV_I] map_sum.simps
     map_prod_simp sum_set_simps prod_set_simps cSup_singleton Un_empty_left Un_empty_right
-    Union_empty image_insert image_empty map_Type_pre_def id_def)
+    Union_empty image_insert image_empty map_sftypeP_pre_def id_def)
   apply (rule exI[of _ \<sigma>])
   apply (rule conjI assms)+
    apply (unfold id_on_def atomize_all atomize_imp)[1]
@@ -88,28 +88,28 @@ lemma Forall_rrename:
   apply (rule refl)
   done
 
-lemma Forall_swap: "y \<notin> FFVars_Type T2 - {x} \<Longrightarrow> Forall (x::'a::var_Type_pre) T1 T2 = Forall y T1 (rrename_Type (id(x:=y,y:=x)) T2)"
+lemma Forall_swap: "y \<notin> FFVars_sftypeP T2 - {x} \<Longrightarrow> Forall (x::'a::var_sftypeP_pre) T1 T2 = Forall y T1 (rrename_sftypeP (id(x:=y,y:=x)) T2)"
   apply (rule trans)
    apply (rule Forall_rrename)
      apply (rule bij_swap[of x y])
     apply (rule supp_swap_bound)
-    apply (rule cinfinite_imp_infinite[OF Type.UNIV_cinfinite])
+    apply (rule cinfinite_imp_infinite[OF sftypeP.UNIV_cinfinite])
   by auto
 
 (* Monomorphising: *)
-instance var :: var_Type_pre apply standard
+instance var :: var_sftypeP_pre apply standard
   using Field_natLeq infinite_iff_card_of_nat infinite_var
   by (auto simp add: regularCard_var)
 
-type_synonym type = "var Type"
-type_synonym \<Gamma>\<^sub>\<tau> = "(var \<times> type) list"
+type_synonym sftype = "var sftypeP"
+type_synonym \<Gamma>\<^sub>\<tau> = "(var \<times> sftype) list"
 
 definition map_context :: "(var \<Rightarrow> var) \<Rightarrow> \<Gamma>\<^sub>\<tau> \<Rightarrow> \<Gamma>\<^sub>\<tau>" where
-  "map_context f \<equiv> map (map_prod f (rrename_Type f))"
+  "map_context f \<equiv> map (map_prod f (rrename_sftypeP f))"
 
 abbreviation FFVars_ctxt :: "\<Gamma>\<^sub>\<tau> \<Rightarrow> var set" where
-  "FFVars_ctxt xs \<equiv> \<Union>(FFVars_Type ` snd ` set xs)"
-abbreviation extend :: "\<Gamma>\<^sub>\<tau> \<Rightarrow> var \<Rightarrow> type \<Rightarrow> \<Gamma>\<^sub>\<tau>" ("_ ,, _ <: _" [57,75,75] 71) where
+  "FFVars_ctxt xs \<equiv> \<Union>(FFVars_sftypeP ` snd ` set xs)"
+abbreviation extend :: "\<Gamma>\<^sub>\<tau> \<Rightarrow> var \<Rightarrow> sftype \<Rightarrow> \<Gamma>\<^sub>\<tau>" ("_ ,, _ <: _" [57,75,75] 71) where
   "extend \<Gamma> x T \<equiv> (x, T)#\<Gamma>"
 abbreviation concat :: "\<Gamma>\<^sub>\<tau> \<Rightarrow> \<Gamma>\<^sub>\<tau> \<Rightarrow> \<Gamma>\<^sub>\<tau>" (infixl "(,,)" 71) where
   "concat \<Gamma> \<Delta> \<equiv> \<Delta> @ \<Gamma>"
@@ -126,7 +126,7 @@ lemma map_context_comp0[simp]:
   shows "map_context f \<circ> map_context g = map_context (f \<circ> g)"
   apply (rule ext)
   unfolding map_context_def
-  using assms by (auto simp: Type.rrename_comps)
+  using assms by (auto simp: sftypeP.rrename_comps)
 
 lemmas map_context_comp = trans[OF comp_apply[symmetric] fun_cong[OF map_context_comp0]]
 declare map_context_comp[simp]
@@ -138,7 +138,7 @@ lemma context_dom_set[simp]:
 lemma set_bd_UNIV: "|set xs| <o |UNIV::var set|"
   apply (rule ordLess_ordLeq_trans)
     apply (tactic \<open>resolve_tac @{context} (BNF_Def.set_bd_of_bnf (the (BNF_Def.bnf_of @{context} @{type_name list}))) 1\<close>)
-  apply (rule var_Type_pre_class.large)
+  apply (rule var_sftypeP_pre_class.large)
   done
 
 lemma context_set_bd_UNIV[simp]: "|dom xs| <o |UNIV::var set|"
@@ -155,18 +155,18 @@ shows "map_context f \<Gamma> = \<Gamma>"
    apply (rule list.map_cong0[of _ _ id])
    apply (rule trans)
     apply (rule prod.map_cong0[of _ _ id _ id])
-  using assms by (fastforce intro!: Type.rrename_cong_ids)+
+  using assms by (fastforce intro!: sftypeP.rrename_cong_ids)+
 
 lemma ls_UNIV_iff_finite: "|A| <o |UNIV::var set| \<longleftrightarrow> finite A"
 using finite_iff_le_card_var by blast
 
-lemma rrename_swap_FFvars[simp]: "X \<notin> FFVars_Type T \<Longrightarrow> Y \<notin> FFVars_Type T \<Longrightarrow>
-  rrename_Type (id(X := Y, Y := X)) T = T"
-apply(rule Type.rrename_cong_ids) by auto
+lemma rrename_swap_FFvars[simp]: "X \<notin> FFVars_sftypeP T \<Longrightarrow> Y \<notin> FFVars_sftypeP T \<Longrightarrow>
+  rrename_sftypeP (id(X := Y, Y := X)) T = T"
+apply(rule sftypeP.rrename_cong_ids) by auto
 
 lemma map_context_swap_FFVars[simp]:
-"\<forall>k\<in>set \<Gamma>. X \<noteq> fst k \<and> X \<notin> FFVars_Type (snd k) \<and>
-           Y \<noteq> fst k \<and> Y \<notin> FFVars_Type (snd k) \<Longrightarrow>
+"\<forall>k\<in>set \<Gamma>. X \<noteq> fst k \<and> X \<notin> FFVars_sftypeP (snd k) \<and>
+           Y \<noteq> fst k \<and> Y \<notin> FFVars_sftypeP (snd k) \<Longrightarrow>
     map_context (id(X := Y, Y := X)) \<Gamma> = \<Gamma>"
   unfolding map_context_def apply(rule map_idI) by auto
 
